Assignment 12

sf/Assignment12_05.v
@@ -12,32 +12,87 @@ Require Export Assignment12_04.
 >>
 *)
 
+Definition f := (Id 0).
+Definition x := (Id 1).
+
 Definition halve : tm :=
-  FILL_IN_HERE.
+  tfix (tabs f (TArrow TNat TNat) 
+    (tabs x TNat (tif0 (tvar x) (tnat 0)
+      (tif0 (tpred (tvar x)) (tnat 0) (tsucc (tapp (tvar f) (tpred (tpred (tvar x))))))))).
 
 Example halve_type: empty |- halve \in TArrow TNat TNat.
 Proof.
-  (* unfold halve; eauto 10. *)
-  exact FILL_IN_HERE.
+  unfold halve; eauto 10.
 Qed.
 
 Example halve_10: tapp halve (tnat 10) ==>* tnat 5.
 Proof.
-  (* unfold halve; normalize. *)
-  exact FILL_IN_HERE.
+  unfold halve; normalize.
 Qed.
 
 Example halve_11: tapp halve (tnat 11) ==>* tnat 5.
 Proof.
-  (* unfold halve; normalize. *)
-  exact FILL_IN_HERE.
+  unfold halve; normalize.
 Qed.
 
 
 Theorem halve_correct: forall n,
    tapp halve (tnat (n+n)) ==>* tnat n.
 Proof.
-  exact FILL_IN_HERE.
+  unfold halve.
+  intros.
+  induction n.
+  normalize.
+  eapply multi_step.
+  eapply ST_AppFix; eauto.
+  eapply multi_step.
+  eapply ST_App1.
+  eapply ST_AppAbs.
+  eauto.
+  simpl.
+  eapply multi_step.
+  eapply ST_AppAbs.
+  eauto.
+  simpl.
+  eapply multi_step.
+  apply ST_If0Nonzero.
+  eapply multi_step.
+  apply ST_If01.
+  apply ST_PredNat.
+  simpl.
+  rewrite plus_comm.
+  simpl.
+  eapply multi_step.
+  apply ST_If0Nonzero.
+  eapply multi_step.
+  apply ST_Succ1.
+  apply ST_App2.
+  auto.
+  apply ST_Pred.
+  apply ST_PredNat.
+  eapply multi_step.
+  apply ST_Succ1.
+  apply ST_App2.
+  auto.
+  apply ST_PredNat.
+  simpl.
+  apply multi_trans with (tsucc (tnat n)).
+  Lemma tsucc_multi: forall t t',
+    t ==>* t' -> tsucc t ==>* tsucc t'.
+  Proof.
+    intros.
+    induction H.
+    auto.
+    apply multi_step with (tsucc y).
+    apply ST_Succ1.
+    assumption.
+    assumption.
+  Qed.
+  apply tsucc_multi.
+  assumption.
+  eapply multi_step.
+  apply ST_SuccNat.
+  auto.
 Qed.
 
 (*-- Check --*)
